A12Kernel.lean
@@ -187,6 +187,7 @@ import A12Kernel.Elaboration.AddressedFullDateFirstFilledComputation
 import A12Kernel.Elaboration.AddressedFullDateFirstFilledFormalInput
 import A12Kernel.Elaboration.TimeFirstFilledComputation
 import A12Kernel.Elaboration.AddressedTimeFirstFilledComputation
+import A12Kernel.Elaboration.AddressedTimeFirstFilledFormalInput
 import A12Kernel.Elaboration.StarGroup
 import A12Kernel.Elaboration.StarNumber
 import A12Kernel.Elaboration.NumberEntityValueList
